copied all needed definitions

OrderedRecSubtyping-STLC.v
@@ -654,6 +654,954 @@ Module Declarative.
         End InvSubsumption.
     End Subtype.
     Export Subtype.
+
+    Module Checks.
+        (* Static Semantics with Subsumption *)
+        Inductive check (g : gamma) : expr -> type -> Prop :=
+            | check_subsume : forall (e : expr) (u v : type),
+                subtype u v ->
+                check g e u ->
+                check g e v
+            | check_unit :
+                check g EUnit TUnit
+            | check_var : forall (x : id) (t : type),
+                g x = Some t ->
+                check g (EVar x) t
+            | check_fun : forall (x : id) (u v : type) (e : expr),
+                check (bind x u g) e v ->
+                check g (EFun x u e) (TFun u v)
+            | check_app : forall (e1 e2 : expr) (u v : type),
+                check g e1 (TFun u v) ->
+                check g e2 u ->
+                check g (EApp e1 e2) v
+            | check_rec : forall (es : fields expr) (ts : fields type),
+                nodupfs es -> nodupfs ts ->
+                relfs (check g) es ts ->
+                check g (ERec es) (TRec ts)
+            | check_prj : forall (e : expr) (x : id) (t : type) (ts : fields type),
+                In (x,t) ts ->
+                check g e (TRec ts) ->
+                check g (EPrj e x) t.
+
+        Section CheckInduction.
+            Variable P : @gamma type -> expr -> type -> Prop.
+
+            Hypothesis HSubsume : 
+                forall (g : gamma) (e : expr) (u v : type),
+                subtype u v -> check g e u -> P g e u -> P g e v.
+
+            Hypothesis HUnit : 
+                forall (g : gamma), P g EUnit TUnit.
+
+            Hypothesis HVar :
+                forall (g : gamma) (x : id) (t : type),
+                g x = Some t -> 
+                P g (EVar x) t.
+
+            Hypothesis HFun :
+                forall (g : gamma) (x : id) (u v : type) (e : expr),
+                check (bind x u g) e v ->
+                P (bind x u g) e v ->
+                P g (EFun x u e) (TFun u v).
+
+            Hypothesis HApp :
+                forall (g : gamma) (e1 e2 : expr) (u v : type),
+                check g e1 (TFun u v) ->
+                P g e1 (TFun u v) ->
+                check g e2 u ->
+                P g e2 u ->
+                P g (EApp e1 e2) v.
+
+            Hypothesis HRec :
+                forall (g : gamma) (es : fields expr) (ts : fields type),
+                nodupfs es -> nodupfs ts ->
+                relfs (check g) es ts ->
+                relfs (P g) es ts ->
+                P g (ERec es) (TRec ts).
+
+            Hypothesis HPrj :
+                forall (g : gamma) (e : expr) (x : id) (t : type) (ts : fields type),
+                In (x,t) ts ->
+                check g e (TRec ts) ->
+                P g e (TRec ts) ->
+                P g (EPrj e x) t.
+
+            Fixpoint IHCheck (g : gamma) (e : expr) (t : type) (HC :check g e t) : P g e t :=
+                match HC in check _ e' t' return (P g e' t') with
+                | check_subsume _ e u v HSuv HCeu => 
+                    HSubsume g e u v HSuv HCeu (IHCheck g e u HCeu)
+                | check_unit _ => HUnit g
+                | check_var _ x t HB => HVar g x t HB
+                | check_fun _ x u v e HCev =>
+                    HFun g x u v e HCev (IHCheck (bind x u g) e v HCev)
+                | check_app _ e1 e2 u v HCe1uv HCe2u =>
+                    HApp g e1 e2 u v 
+                        HCe1uv (IHCheck g e1 (TFun u v) HCe1uv)
+                        HCe2u (IHCheck g e2 u HCe2u)
+                | check_rec _ es ts NDes NDts HRs =>
+                    let fix rec_help {es' : fields expr} {ts' : fields type}
+                        (HRs' : relfs (check g) es' ts') : Forall2 (relf (P g)) es' ts' :=
+                        match HRs' in (Forall2 _ le lt) 
+                            return (Forall2 (relf (P g)) le lt) with
+                        | Forall2_nil _ => Forall2_nil (relf (P g))
+                        | Forall2_cons e t Het Hests =>
+                            Forall2_cons
+                                e t (relf_pred (IHCheck g) Het) 
+                                (rec_help Hests)
+                        end in
+                    HRec g es ts NDes NDts HRs (rec_help HRs)
+                | check_prj _ e x t ts Hints HCets =>
+                    HPrj g e x t ts Hints HCets (IHCheck g e (TRec ts) HCets)
+                end.
+        End CheckInduction.
+
+        Definition checks : expr -> type -> Prop := check empty.
+
+        Example benjy : 
+            checks 
+                (EApp 
+                    (EFun "r" (TRec [("x",TUnit)]) 
+                        (EPrj (EVar "r") "x")) 
+                    (ERec [("x",EUnit);("y",EUnit)]))
+                TUnit.
+        Proof.
+            apply check_app with (u := TRec [("x",TUnit)]).
+            - apply check_fun. apply check_prj with 
+                (ts := [("x",TUnit)]);
+                constructor; reflexivity.
+            - apply check_subsume with 
+                (u := TRec [("x", TUnit);("y",TUnit)]).
+                + apply st_rec_width with
+                    (us := [("x",TUnit)])
+                    (vs := [("y",TUnit)]).
+                + apply check_rec.
+                    { constructor; try constructor;
+                        try constructor; 
+                        try intros DUMB; inv DUMB;
+                        try discriminate. inv H. }
+                    { constructor; try constructor;
+                        try constructor; 
+                        try intros DUMB; inv DUMB;
+                        try discriminate. inv H. }
+                    { constructor.
+                        - split; try reflexivity. constructor. 
+                        - constructor.
+                            + split.
+                                * reflexivity.
+                                * constructor.
+                            + constructor. }
+        Qed. 
+
+        (* Inversion on the Typing Relation. *)
+        Section InvCheck.
+            Lemma st_fields_name :
+                forall (us ws : fields type),
+                subtype (TRec us) (TRec ws) ->
+                forall (x : id) (w : type),
+                In (x,w) ws ->
+                exists (u : type),
+                In (x,u) us /\ subtype u w.
+            Proof.
+                intros us ws HS.
+                dependent induction HS using IHSubtype; intros x w Hinws.
+                - subst. exists w. 
+                    split; auto. constructor.
+                - assert (HSusws : subtype (TRec us) (TRec ws)).
+                    + apply st_trans with (u := u); assumption.
+                    + pose proof inv_rec u ws HS2 as [vs [Huvs HSvws]]. subst.
+                        assert (Hduhu : TRec us = TRec us);
+                        assert (Hduhv : TRec vs = TRec vs);
+                        assert (Hduhw : TRec ws = TRec ws);
+                        try reflexivity.
+                        pose proof IHHS2 vs ws Hduhv Hduhw x w as IH2.
+                        apply IH2 in Hinws as [w' [Hinvs HSw'w]].
+                        pose proof IHHS1 us vs Hduhu Hduhv x w' as IH1.
+                        apply IH1 in Hinvs as [u' [Hinus Hsubu'w']].
+                        exists u'. split; try assumption.
+                        apply st_trans with (u := w');
+                        assumption.
+                - exists w. split.
+                    + apply in_or_app.
+                        left. auto.
+                    + constructor.
+                - induction H0; inv Hinws.
+                    + inv H. inv H5. destruct x0 as [x0 u0].
+                        exists u0. split.
+                        * constructor. simpl in H2.
+                            rewrite <- H2. reflexivity.
+                        * assumption.
+                    + inv H. pose proof IHForall2 H8 H2 as HEX.
+                        destruct HEX as [u [Hinl HSuw]].
+                        exists u. split; try assumption.
+                        apply in_cons. assumption.
+            Qed.
+
+            Lemma rec_fields_name :
+                forall (es : fields expr) (ts : fields type),
+                relfs checks es ts ->
+                forall (x : id) (t : type),
+                In (x,t) ts ->
+                exists (e : expr), In (x,e) es.
+            Proof.
+                intros es ts HR. induction HR;
+                intros z t Hints.
+                - inv Hints.
+                - destruct x as (x,e). inv Hints.
+                    + exists e. constructor.
+                        unfold relf in H.
+                        destruct H as [HF _].
+                        simpl in *. subst.
+                        reflexivity.
+                    + apply IHHR in H0 as [e' Hinl].
+                        exists e'. apply in_cons.
+                        assumption.
+            Qed.
+
+            Lemma inv_chk_fun :
+                forall (g : gamma) (t u v : type) (x : id) (e : expr),
+                check g (EFun x t e) (TFun u v) ->
+                subtype u t /\ check (bind x t g) e v.
+            Proof.
+                intros g t u v x e HC. 
+                dependent induction HC using IHCheck.
+                - pose proof inv_fun u0 u v H as [a [b [Huab [Hua Hbv]]]].
+                    subst. assert (HEFun : EFun x t e = EFun x t e);
+                    assert (HTFun : TFun a b = TFun a b); try reflexivity.
+                    pose proof IHHC t a b x e HEFun HTFun as IH.
+                    destruct IH as [HS HCB]. split.
+                    + apply st_trans with (u := a); assumption.
+                    + apply check_subsume with (u := b); assumption.
+                - split; try apply st_refl. assumption.
+            Qed.
+
+            Lemma inv_chk_rec :
+                forall (g : gamma) (es : fields expr) (ts : fields type),
+                check g (ERec es) (TRec ts) ->
+                forall (x : id) (t : type),
+                In (x,t) ts ->
+                exists (e : expr), 
+                In (x,e) es /\ check g e t.
+            Proof.
+                intros g es ts HC x t Hints.
+                dependent induction HC using IHCheck.
+                - pose proof inv_rec u ts H as HRu.
+                    destruct HRu as [us [Huus HSus]].
+                    assert (HERec : ERec es = ERec es);
+                    try reflexivity.
+                    pose proof st_fields_name us ts HSus x t Hints as HT.
+                    destruct HT as [w [Hinus HSut]].
+                    pose proof IHHC es us HERec Huus x w Hinus as IH.
+                    destruct IH as [e [Hines HCew]]. exists e. split.
+                    + assumption.
+                    + apply check_subsume with (u := w);
+                        assumption.
+                - induction H2; inv Hints;
+                    inv H; inv H0; clear H; clear H0;
+                    inv H1; clear H1.
+                    + destruct x0 as [x0 e0]. exists e0. 
+                        destruct H5 as [Hfst Hck].
+                        simpl in *; subst. split.
+                        * left. reflexivity.
+                        * assumption.
+                    + pose proof IHForall2 H8 H10 H12 H4 as IH. 
+                        destruct IH as [e [HIN HCK]].
+                        exists e. split; try assumption.
+                        apply in_cons. assumption.
+            Qed.
+
+            Lemma inv_chk_rec' :
+                forall (g : gamma) (es : fields expr) (ts : fields type),
+                check g (ERec es) (TRec ts) ->
+                forall (x : id) (t : type),
+                In (x,t) ts ->
+                forall (e : expr),
+                In (x,e) es ->
+                check g e t.
+            Proof.
+                intros g es ts HC x t Hints.
+                intros f Hinfes.
+                dependent induction HC using IHCheck.
+                - apply inv_rec in H as [us [Huus HSusts]].
+                    pose proof st_fields_name 
+                        us ts HSusts x t Hints as SFN.
+                    destruct SFN as [w [Hinus HSwt]].
+                    apply check_subsume with (u := w); auto.
+                    apply IHHC with (es0 := es) (ts := us) (x := x);
+                    auto. 
+                - assert (HC : check g (ERec es) (TRec ts)).
+                    + constructor; auto.
+                    + pose proof inv_chk_rec g es ts 
+                        HC x t Hints as ICR.
+                        destruct ICR as [e [Hin Hget]].
+                        pose proof relfs_nodup_eq es x e f 
+                            H Hin Hinfes as EF. subst.
+                            assumption.                  
+            Qed.
+        End InvCheck.
+    End Checks.
+    Export Checks.
+
+    Module Value.
+        Inductive value : expr -> Prop :=
+            | value_unit : value EUnit
+            | value_fun : forall (x : id) (t : type) (e : expr),
+                value (EFun x t e)
+            | value_rec : forall (vs : fields expr),
+                predfs value vs ->
+                value (ERec vs).
+
+        Section ValueDec.
+            Fixpoint value_dec (v : expr) : {value v} + {~ value v}. 
+            Proof.
+                destruct v.
+                - left. constructor.
+                - right. intros HF. inv HF.
+                - left. constructor.
+                - right. intros HF. inv HF.
+                - induction fs.
+                    + left. constructor. constructor.
+                    + destruct (value_dec (snd a)) as [AV | AV].
+                        { destruct IHfs as [V | V].
+                            - pose proof 
+                                (fun x : field expr => value_dec (snd x)) as PFV.
+                                pose proof @Forall_dec
+                                    (field expr) (predf value) 
+                                    PFV fs as FD.
+                                destruct FD as [FV | FV].
+                                + left. constructor. 
+                                    constructor; assumption.
+                                + right. intros HF. apply FV.
+                                    inv HF. inv H0. assumption.
+                            - right. intros HF. apply V. 
+                                inv HF. inv H0. constructor.
+                                assumption. }
+                        { right. intros HF. apply AV. inv HF.
+                            inv H0. assumption. }
+                - right. intros HF. inv HF.
+            Qed.
+        End ValueDec.
+    End Value.
+    Export Value.
+
+    Module Step.
+        (* free variables *)
+        Fixpoint fv (e : expr) : IS.t :=
+            match e with
+            | EUnit => IS.empty
+            | EVar x => IS.singleton x
+            | EFun x _ e => IS.remove x (fv e)
+            | EApp e1 e2 => IS.union (fv e1) (fv e2)
+            | ERec (es) => 
+                fold_right 
+                    (fun (e : field expr) acc => 
+                        IS.union acc (fv (snd e)))
+                    IS.empty es
+            | EPrj e _ => fv e
+            end.
+
+        (* Capture-avoiding Substitution *)
+        Inductive sub (x : id) (es : expr) : expr -> expr -> Prop :=
+            | sub_unit : sub x es EUnit EUnit
+            | sub_hit : sub x es (EVar x) es
+            | sub_miss : forall (y : id), 
+                x <> y -> 
+                sub x es (EVar y) (EVar y)
+            | sub_fun_bound : forall (t : type) (e : expr),
+                sub x es (EFun x t e) (EFun x t e)
+            | sub_fun_notfree : forall (y : string) (t : type) (e e' : expr),
+                x <> y ->
+                ~ IS.In y (fv es) -> 
+                sub x es e e' -> 
+                sub x es (EFun y t e) (EFun y t e')
+            | sub_fun_free : forall (y z : id) (t : type) (e e' e'' : expr),
+                x <> y -> 
+                x <> z -> 
+                y <> z ->
+                IS.In y (fv es) -> 
+                ~ IS.In z (fv es) ->
+                ~ IS.In z (fv e) ->
+                sub y (EVar z) e e' -> 
+                sub x es e' e'' -> 
+                sub x es (EFun y t e) (EFun z t e'')
+            | sub_app : forall (e1 e1' e2 e2' : expr),
+                sub x es e1 e1' -> 
+                sub x es e2 e2' -> 
+                sub x es (EApp e1 e2) (EApp e1' e2')
+            | sub_rec : forall (fs fs' : fields expr),
+                relfs (sub x es) fs fs' ->
+                sub x es (ERec fs) (ERec fs')
+            | sub_prj : forall (e e' : expr) (y : id),
+                sub x es e e' ->
+                sub x es (EPrj e y) (EPrj e' y).
+
+        Section SubstitutionInduction.
+            Variable P : id -> expr -> expr -> expr -> Prop.
+
+            Hypothesis HUnit : 
+                forall (x : id) (es : expr), 
+                P x es EUnit EUnit.
+
+            Hypothesis HHit : 
+                forall (x : id) (es : expr),
+                P x es (EVar x) es.
+
+            Hypothesis HMiss : 
+                forall (x : id) (es : expr) (y : id),
+                x <> y -> P x es (EVar y) (EVar y).
+
+            Hypothesis HFunBound : 
+                forall (x : id) (es : expr) (t : type) (e : expr),
+                P x es (EFun x t e) (EFun x t e).
+
+            Hypothesis HFunNotFree : 
+                forall (x : id) (es : expr) (y : string) (t : type) (e e' : expr),
+                x <> y -> ~ IS.In y (fv es) ->
+                sub x es e e' -> P x es e e' -> 
+                P x es (EFun y t e) (EFun y t e').
+
+            Hypothesis HFunFree :
+                forall (x : id) (es : expr) (y z : id)
+                (t : type) (e e' e'' : expr),
+                x <> y -> x <> z ->
+                y <> z -> IS.In y (fv es) ->
+                ~ IS.In z (fv es) -> ~ IS.In z (fv e) ->
+                sub y (EVar z) e e' -> P y (EVar z) e e' ->
+                sub x es e' e'' -> P x es e' e'' -> 
+                P x es (EFun y t e) (EFun z t e'').
+
+            Hypothesis HApp :
+                forall (x : id) (es e1 e1' e2 e2' : expr),
+                sub x es e1 e1' -> P x es e1 e1' ->
+                sub x es e2 e2' -> P x es e2 e2' -> 
+                P x es (EApp e1 e2) (EApp e1' e2').
+
+            Hypothesis HRec : 
+                forall (x : id) (es : expr) (fs fs' : fields expr),
+                relfs (sub x es) fs fs' -> 
+                relfs (P x es) fs fs' ->
+                P x es (ERec fs) (ERec fs').
+
+            Hypothesis HPrj :
+                forall (x : id) (es e e' : expr) (y : id),
+                sub x es e e' -> P x es e e' -> 
+                P x es (EPrj e y) (EPrj e' y).
+
+            Fixpoint IHSubstitute (x : id) (es e e' : expr)
+            (HS : sub x es e e') {struct HS} : P x es e e' :=
+                match HS in sub _ _ pe pe' return P x es pe pe' with
+                | sub_unit _ _ => HUnit x es
+                | sub_hit _ _ => HHit x es
+                | sub_miss _ _ y Hxy => HMiss x es y Hxy
+                | sub_fun_bound _ _ t e => HFunBound x es t e
+                | sub_fun_notfree _ _ y t e e' Hxy Hines HS =>
+                    HFunNotFree x es y t e e' 
+                        Hxy Hines HS (IHSubstitute x es e e' HS)
+                | sub_fun_free _ _ y z t e e' e'' 
+                    Hxy Hxz Hyz Hinyes Hinzes Hinze HSee' HSe'e'' =>
+                    HFunFree x es y z t e e' e'' 
+                        Hxy Hxz Hyz Hinyes Hinzes Hinze
+                        HSee' (IHSubstitute y (EVar z) e e' HSee')
+                        HSe'e'' (IHSubstitute x es e' e'' HSe'e'')
+                | sub_app _ _ e1 e1' e2 e2' HS1 HS2 =>
+                    HApp x es e1 e1' e2 e2'
+                        HS1 (IHSubstitute x es e1 e1' HS1)
+                        HS2 (IHSubstitute x es e2 e2' HS2)
+                | sub_rec _ _ fs fs' HRs =>
+                    let fix rec_help {fds : fields expr} {fds' : fields expr}
+                    (HRs' : relfs (sub x es) fds fds') : Forall2 (relf (P x es)) fds fds' :=
+                        match HRs' in (Forall2 _ l l') 
+                            return (Forall2 (relf (P x es)) l l') with
+                        | Forall2_nil _ => Forall2_nil (relf (P x es))
+                        | Forall2_cons fd fd' HRhead HRtail =>
+                            Forall2_cons
+                                fd fd' (relf_pred (IHSubstitute x es) HRhead) 
+                                (rec_help HRtail)
+                        end in
+                    HRec x es fs fs' HRs (rec_help HRs)
+                | sub_prj _ _ e e' y HS =>
+                    HPrj x es e e' y HS (IHSubstitute x es e e' HS)
+                end.
+        End SubstitutionInduction.
+
+        Axiom sub_exists : forall (x : id) (s e : expr), exists e', sub x s e e'.
+
+        (* Dynamic Semantics *)
+        Inductive step : expr -> expr -> Prop :=
+            | step_redux : forall (x : id) (t : type) (e es e' : expr),
+                sub x es e e' ->
+                step (EApp (EFun x t e) es) e'
+            | step_app : forall (e1 e2 e1' : expr),
+                step e1 e1' ->
+                step (EApp e1 e2) (EApp e1' e2)
+            | step_prj_rec : forall (es : fields expr) (x : id) (e : expr),
+                In (x,e) es ->
+                step (EPrj (ERec es) x) e
+            | step_prj : forall (e e' : expr) (x : id),
+                step e e' ->
+                step (EPrj e x) (EPrj e' x)
+            | step_rec : forall (vs es : fields expr) (x : id) (e e' : expr),
+                predfs value vs ->
+                step e e' ->
+                step (ERec (vs ++ (x,e) :: es)) (ERec (vs ++ (x,e') :: es)).
+    End Step.
+    Export Step.
+
+    Section CanonicalForms.
+        Definition canon_unit (v : expr) : Prop :=
+            value v -> checks v TUnit -> v = EUnit.
+
+        Definition canon_fun (v : expr) : Prop :=
+            forall (a b : type),
+            value v -> checks v (TFun a b) -> 
+            exists (x : id) (t : type) (e : expr), 
+            subtype a t /\ v = EFun x t e.
+
+        Definition canon_rec (v : expr) := 
+            forall (ts : fields type),
+            value v -> checks v (TRec ts) ->
+            exists (es : fields expr) (us : fields type), 
+            v = ERec es /\
+            relfs (check empty) es us /\ 
+            subtype (TRec us) (TRec ts).
+
+        Lemma canonical_forms_unit : 
+            forall (v : expr), canon_unit v.
+        Proof.
+            unfold canon_unit. intros v HV HChk;
+            dependent induction HChk.
+            - apply inv_unit in H as HU. auto.
+            - reflexivity.
+            - inversion HV.
+            - inversion HV.
+            - inversion HV.
+        Qed.
+
+        Lemma canonical_forms_fun :
+            forall (v : expr), canon_fun v.
+        Proof.
+            unfold canon_fun. intros v t t' HV HChk.
+            dependent induction HChk.
+            - apply inv_fun in H as HU.
+                destruct HU as [a' [b' [HF [HSA HSB]]]].
+                specialize IHHChk with
+                    (t := a') (t' := b').
+                pose proof (IHHChk HV HF) as IH.
+                destruct IH as [x [w [e' [HSW HFW]]]].
+                exists x. exists w. exists e'. split.
+                + apply st_trans with
+                    (t := t) (u := a') (v := w);
+                    assumption.
+                + assumption.
+            - inversion HV.
+            - exists x. exists t. exists e. 
+                split; constructor.
+            - inversion HV.
+            - inversion HV.
+        Qed.
+
+        Lemma canonical_forms_rec :
+            forall (v : expr), canon_rec v.
+        Proof.
+            unfold canon_rec. intros v ts HV HChk.
+            dependent induction HChk.
+            - apply inv_rec in H as [us [HU HSusts]].
+                specialize IHHChk with (ts := us).
+                apply IHHChk in HV as IH; auto.
+                destruct IH as [es [vs [Hrec [HR HSvsus]]]].
+                exists es. exists vs. split; auto. split; auto.
+                apply st_trans with
+                    (t := (TRec vs)) (u := (TRec us)) (v := (TRec ts));
+                assumption.
+            - inv HV.
+            - inv HV.
+            - exists es. exists ts. 
+                split; try reflexivity.
+                induction HV; subst; constructor;
+                try assumption;
+                try apply st_refl.
+            - inv HV. 
+        Qed.
+    End CanonicalForms.
+
+    Section Progress.
+        Definition progress_thm (e : expr) (t : type) : Prop :=
+            checks e t -> value e \/ exists (e' : expr), step e e'.
+
+        Lemma var_empty_checks :
+            forall (x : id) (t : type),
+            ~ checks (EVar x) t.
+        Proof.
+            intros x t H. unfold checks in *.
+            remember empty as o in H. 
+            remember (EVar x) as z in H.
+            dependent induction H; 
+            auto; try inv Heqz.
+            discriminate.
+        Qed.
+
+        Lemma val_rec_exists :
+            forall (es : fields expr),
+            ~ value (ERec es) <-> Exists (predf (fun e => ~ value e)) es.
+        Proof.
+            intros es. split; intros H.
+            - induction es.
+                + exfalso. apply H.
+                    constructor. constructor.
+                + apply Exists_cons. 
+                    destruct (value_dec (snd a)).
+                    * right. apply IHes. intros V.
+                        inv V. apply H. constructor.
+                        constructor; assumption.
+                    * left. unfold predf. assumption.
+            - intros V. apply Exists_Forall_neg in H.
+                + apply H. inv V. assumption.
+                + pose proof 
+                    (fun x : field expr => 
+                        value_dec (snd x)) as PFV.
+                    intros e. specialize PFV with e.
+                    destruct PFV as [VE | VE]; auto.
+        Qed.
+
+        Lemma val_rec_prefix :
+            forall (es : fields expr),
+            ~ value (ERec es) ->
+            exists (x : id) (e : expr) 
+                (qs rs : fields expr),
+            ~ value e /\ 
+            predfs value qs /\
+            es = qs ++ (x,e) :: rs.
+        Proof.
+            induction es; intros HV.
+            - exfalso. apply HV.
+                constructor. constructor.
+            - destruct (value_dec (snd a)).
+                { assert (HVes : ~ value (ERec es)).
+                    - intros HR. apply HV. inv HR.
+                        constructor.
+                        constructor; assumption.
+                    - pose proof IHes HVes as IH.
+                        destruct IH as [x [e [qs [rs [HNV [HPV Hqer]]]]]].
+                        exists x. exists e. exists (a :: qs). 
+                        exists rs. split; try assumption. split.
+                        + constructor; assumption.
+                        + rewrite <- app_comm_cons.
+                            rewrite Hqer. reflexivity. }
+                { exists (fst a). exists (snd a).
+                    exists []. exists es. split;
+                    try assumption. split.
+                    - constructor.
+                    - rewrite app_nil_l. destruct a as (x,e).
+                        reflexivity. }
+        Qed.
+
+        Theorem Progress :
+            forall (e : expr) (t : type), progress_thm e t.
+        Proof.
+            unfold progress_thm. intros e t HC.
+            unfold checks in *. remember empty as o in HC.
+            dependent induction HC using IHCheck; subst;
+            assert (HE : @empty type = @empty type);
+            try reflexivity.
+            - destruct IHHC as [V | [e' HS]].
+                + reflexivity.
+                + left. assumption.
+                + right. exists e'. assumption.
+            - left. constructor.
+            - discriminate.
+            - left. constructor.
+            - right. pose proof IHHC1 HE as [V | [e1' HS]].
+                + pose proof canonical_forms_fun e1 u v V HC1
+                    as [x [t [e [HS HF]]]].
+                    pose proof sub_exists x e2 e as [e' HSub].
+                    exists e'. subst. constructor. assumption.
+                + exists (EApp e1' e2). constructor. assumption.
+            - induction H2.
+                + left. constructor. constructor.
+                + inv H. inv H1. inv H0. clear H. clear H0. inv H2.
+                    pose proof IHForall2 H7 as IH2.
+                    destruct H2 as [HFXY YES].
+                    pose proof YES HE as [HVX | [e' HSX]].
+                    { destruct (value_dec (ERec l)) as [V | V].
+                        - left. constructor. inv V.
+                            constructor; auto.
+                        - destruct IH2 as [IH2 | IH2]; try contradiction; auto. 
+                            pose proof val_rec_prefix l V as HEX.
+                            destruct HEX as [z [e [qs [rs [HVE [HPV HL]]]]]].
+                            right. subst. destruct IH2 as [e' HS]. inv HS.
+                            exists (ERec (x :: vs ++ (x0,e'0) :: es)).
+                            rewrite app_comm_cons. rewrite app_comm_cons.
+                            constructor; auto.
+                            constructor; auto. }
+                    { right. destruct x as [x e]. simpl in *.
+                        exists (ERec ((x, e') :: l)).
+                        assert (HPV : predfs value []);
+                        try (constructor; constructor).
+                        pose proof step_rec [] l x e e' HPV HSX as HR.
+                        rewrite app_nil_l in HR. rewrite app_nil_l in HR.
+                        assumption. }
+            - right. pose proof IHHC HE as [V | [e' HS]].
+                + pose proof canonical_forms_rec e ts V HC as HCF.
+                    destruct HCF as [es [us [HRec [HR Hsub]]]]; subst.
+                    pose proof st_fields_name us ts Hsub x t H as [u [Hinus HSut]].
+                    pose proof rec_fields_name es us HR x u Hinus as [e' Hines].
+                    exists e'. constructor. assumption.
+                + exists (EPrj e' x). constructor. assumption.
+        Qed.
+    End Progress.
+
+    Section SubstitutionLemma.
+        Lemma bind_unfree_var :
+            forall (e : expr) (x : id) (u v : type) (g : gamma),
+            ~ IS.In x (fv e) ->
+            check g e u <-> check (bind x v g) e u.
+        Proof.
+            intros e x u v g HN. split; intros HC;
+            dependent induction HC using IHCheck.
+            - pose proof IHHC HN as IH.
+                apply check_subsume with (u := u);
+                assumption.
+            - constructor.
+            - constructor. simpl in *.
+                assert (Hxx0 : x <> x0).
+                + intros Hxx0. apply HN. subst.
+                    constructor. reflexivity.
+                + apply bind_complete; assumption.
+            - constructor. destruct (IdDec.eq_dec x x0) as [HX | HX]; subst.
+                + rewrite <- rebind_correct. assumption.
+                + simpl in *. assert (HNin : ~ IS.In x (fv e)).
+                    * intros HNin. apply HN.
+                        apply not_eq_sym in HX.
+                        apply ISF.remove_2; assumption.
+                    * pose proof bind_diff_comm x x0 v u g HX as BDC.
+                        rewrite <- BDC. pose proof IHHC HNin as IH.
+                        assumption.
+            - simpl in *. apply check_app with (u := u).
+                + apply IHHC1. intros H1. apply HN.
+                    apply ISF.union_2. assumption.
+                + apply IHHC2. intros H2. apply HN.
+                    apply ISF.union_3. assumption.
+            - constructor; auto. clear H. clear H0.
+                induction H2;
+                constructor; inv H1; inv H.
+                + split; try assumption. apply H3.
+                    intros Hxx0. apply HN. simpl.
+                    apply ISF.union_3. assumption.
+                + assert (Hxl : ~ IS.In x (fv (ERec l))).
+                    * intros Hxl. apply HN. simpl in *.
+                        apply ISF.union_2. assumption.
+                    * apply (IHForall2 Hxl H7).
+            - simpl in *. apply check_prj with (ts := ts);
+                try assumption. auto.
+            - pose proof IHHC x v g HN as IH.
+                apply check_subsume with (u := u); auto.
+            - constructor.
+            - simpl in *. constructor.
+                assert (Hxx0 : x <> x0).
+                + intros Hxx0. apply HN. subst.
+                    constructor. reflexivity.
+                + apply bind_complete in H; assumption.
+            - constructor. destruct (IdDec.eq_dec x x0) as [HX | HX]; subst.
+                + rewrite <- rebind_correct in HC. assumption.
+                + simpl in *. assert (HNin : ~ IS.In x (fv e)).
+                    * intros HNin. apply HN.
+                        apply not_eq_sym in HX.
+                        apply ISF.remove_2; assumption.
+                    * pose proof bind_diff_comm x x0 v u g HX as BDC.
+                        symmetry in BDC.
+                        pose proof IHHC x v (bind x0 u g) HNin BDC as IH.
+                        apply IH.
+            - simpl in *. apply check_app with (u := u).
+                + apply IHHC1 with (x0 := x) (v1 := v); 
+                    auto. intros H1. apply HN. 
+                    apply ISF.union_2. assumption.
+                + apply IHHC2 with (x0 := x) (v0 := v); 
+                    auto. intros H2. apply HN. 
+                    apply ISF.union_3. assumption.
+            - constructor; auto. induction H2; 
+                constructor; inv H; inv H0;
+                clear H; clear H0; inv H1; inv H2; inv H5.
+                + split; try assumption.
+                    apply H0 with (x1 := x) (v0 := v); auto.
+                    intros Hxx0. apply HN. simpl.
+                    apply ISF.union_3. assumption.
+                + assert (Hxl : ~ IS.In x (fv (ERec l))).
+                    * intros Hxl. apply HN. simpl in *.
+                        apply ISF.union_2. assumption.
+                    * apply (IHForall2 H7 H9 H11 Hxl).
+            - apply check_prj with (ts := ts); auto.
+                simpl in *. assert (HR : bind x v g = bind x v g);
+                try reflexivity. pose proof IHHC x v g HN HR as IH.
+                assumption.
+        Qed.
+
+        Definition substitution_lemma (x : id) (esub e e' : expr) :=
+            sub x esub e e' ->
+            forall (u v : type) (g : gamma),
+            check (bind x u g) e v -> 
+            check g esub u -> 
+            check g e' v.
+
+        Lemma fields_sub_nodups :
+            forall (x : id) (esub : expr) (es es' : fields expr),
+            relfs (sub x esub) es es' ->
+            nodupfs es -> nodupfs es'.
+        Proof.
+            intros x esub es es' HS.
+            induction HS; intros ND.
+            - constructor.
+            - destruct x0 as [x0 ex0].
+                destruct y as [y ey].
+                destruct H as [Hfst Hsub].
+                simpl in *. subst.
+                inv ND.
+                unfold nodupfs in *. simpl in *.
+                constructor; simpl in *; auto.
+                intros Hin. apply H1.
+                pose proof relfs_name_share (sub x esub) as RNS.
+                apply RNS with (x0 := y) in HS. 
+                apply HS. assumption.
+        Qed.
+
+        Lemma SubstitutionLem :
+            forall (x : id) (esub e e' : expr),
+            substitution_lemma x esub e e'.
+        Proof.
+            intros x esub e e' HS.
+            induction HS using IHSubstitute;
+            intros u v g HCB;
+            remember g as g' in HCB; 
+            dependent induction HCB; intros HC;
+            try (apply check_subsume with (u := u0); auto;
+                apply IHHCB with (x0 := x) (u1 := u) (g' := g); 
+                try reflexivity; assumption);
+            assert (Hgg : g = g); try reflexivity.
+            - constructor.
+            - rewrite bind_correct in H. injintrosubst H. auto.
+            - apply bind_complete in H0 as BC; auto.
+                constructor. auto.
+            - constructor. clear IHHCB. 
+                rewrite <- rebind_correct in HCB.
+                assumption.
+            - pose proof IHHCB g Hgg u e t y 
+                H0 x H HS IHHS as IH.
+                apply check_subsume with (u := u0); auto.
+            - clear IHHCB. constructor.
+                rewrite <- (bind_diff_comm x y u t g H) in HCB.
+                apply IHHS in HCB as IH; auto.
+                apply bind_unfree_var; auto.
+            - pose proof IHHCB g Hgg u H3 e H4 t y 
+                H1 H2 HS1 IHHS1 x H H0 HS2 IHHS2 as IH.
+                apply check_subsume with (u := u0); auto.
+            - clear IHHCB. constructor.
+                apply IHHS2 with (u := u).
+                { apply IHHS1 with (u := t).
+                    - pose proof bind_diff_comm 
+                        x z u t g H0 as BDC1.
+                        rewrite BDC1.
+                        pose proof bind_diff_comm
+                            y z t t (bind x u g) H1 as BDC2.
+                        rewrite BDC2. apply bind_unfree_var; auto.
+                    - apply bind_unfree_var.
+                        + intros Hin. simpl in *.
+                            apply IS.singleton_spec in Hin.
+                            contradiction.
+                        + constructor. apply bind_correct. }
+                { apply bind_unfree_var; auto. }
+            - pose proof IHHCB x e1 e2 HS1 HS2
+                IHHS1 IHHS2 u g as IH.
+                apply check_subsume with (u := u0); auto.
+            - clear IHHCB1. clear IHHCB2.
+                apply check_app with (u := u0).
+                + apply IHHS1 with (u := u); auto.
+                + apply IHHS2 with (u := u); auto.
+            - pose proof IHHCB x fs H H0 u g as IH.
+                apply check_subsume with (u := u0); auto. 
+            - apply check_rec; auto.
+                + apply fields_sub_nodups in H; auto.
+                + generalize dependent fs'.
+                induction H1; intros fs';
+                intros HSfs; intros Hbig;
+                inv HSfs; constructor; auto;
+                destruct x0 as [x0 ex0];
+                destruct y as [y ey];
+                destruct y0 as [y0 ey0];
+                destruct H5 as [Hfst Hsub];
+                inv HSfs; clear HSfs;
+                inv Hbig; clear Hbig;
+                destruct H8 as [Hfst' Hck];
+                destruct H as [Hyy0 Hcky];
+                simpl in *; subst; clear Hfst'.
+                * split; auto; simpl. 
+                    apply Hck with (u := u); auto.
+                * inv H2; clear H2.
+                    inv H3; clear H3. clear H4. clear H2.
+                    pose proof IHForall2 H5 H8
+                        l'0 H9 H11 as IH; clear IHForall2.
+                    apply IH.
+            - pose proof IHHCB x e y HS  IHHS u g as IH.
+                apply check_subsume with (u := u0); auto.
+            - clear IHHCB. apply check_prj with (ts := ts); auto.
+                apply IHHS in HCB as IH; auto.
+        Qed.
+    End SubstitutionLemma.
+
+    Section Preservation.
+        Definition preservation (e e' : expr) : Prop :=
+            step e e' -> forall (t : type),
+            checks e t -> checks e' t.
+
+        Theorem Preservation :
+            forall (e e' : expr), preservation e e'.
+        Proof.
+            intros e e' HS.
+            dependent induction HS; intros u HC;
+            unfold checks in *;
+            remember empty as o in HC.
+            - dependent induction HC.
+                + apply check_subsume with (u := u); auto.
+                    apply IHHC with (x0 := x) (t0 := t)
+                    (e0 := e) (es0 := es); auto.
+                + clear IHHC1. clear IHHC2.
+                    apply inv_chk_fun in HC1 as [HSut Hev].
+                    apply SubstitutionLem in H as SL.
+                    apply SL with (u := t); auto.
+                    apply check_subsume with (u := u); auto.
+            - dependent induction HC.
+                + apply check_subsume with (u := u); auto.
+                    apply IHHC with (e3 := e1) (e4 := e2); auto.
+                + clear IHHC1. clear IHHC2.
+                    apply check_app with (u := u); auto.
+            - generalize dependent e.
+                dependent induction HC;
+                intros e Hin.
+                + apply check_subsume with (u := u); auto.
+                    apply IHHC with (es0 := es) (x0 := x); auto.
+                + clear IHHC.
+                    pose proof inv_chk_rec' empty 
+                        es ts HC x t H e Hin as ICR.
+                    assumption.
+            - dependent induction HC.
+                + apply check_subsume with (u := u); auto.
+                    apply IHHC with (e0 := e) (x0 := x); auto.
+                + clear IHHC. apply check_prj with (ts := ts); auto.
+            - dependent induction HC.
+                { apply check_subsume with (u := u); auto.
+                    apply IHHC with (e0 := e) 
+                        (x0 := x) (es0 := es) (vs0 := vs); auto. }
+                { constructor; auto.
+                    - unfold nodupfs in *.
+                        rewrite map_app.
+                        rewrite map_app in H2.
+                        simpl in *. assumption.
+                    - apply relfs_app in H1 as RA.
+                        destruct RA as [ts1 [ts2 [Hts [Hts1 Hts2]]]].
+                        subst. inv Hts2.
+                        inv H5. apply IHHS in H4.
+                        apply relfs_app_dist; auto.
+                        constructor; auto.
+                        constructor; auto. }
+        Qed.
+    End Preservation.
 End Declarative.
 
 Module Algorithmic.
@@ -798,5 +1746,28 @@ Module Algorithmic.
                 as [nt Hnt]. rewrite Hnt. omega.
         Qed.
         Solve All Obligations with oblige.
+
+        Fixpoint subtype_dec (s t : type) :
+            subtype s t <-> is_subtype s t = true.
+        Proof.
+            destruct s; destruct t;
+            split; intros HY;
+            try reflexivity;
+            try discriminate;
+            try apply st_top;
+            try constructor;
+            try inv HY.
+            - apply subtype_dec in H2.
+                apply subtype_dec in H4.
+                unfold is_subtype. cbn.
+            (* - unfold is_subtype. cbn.
+                destruct fs; reflexivity.
+            - clear H0. 
+                unfold is_subtype in HY.
+                cbn in HY.
+                destruct fs; simpl in HY;
+                discriminate.
+            - *)
+        Admitted.
     End Subtype.
 End Algorithmic.
